powerpc/PrintAsm.ml
@@ -111,7 +111,13 @@ let constant oc cst =
           fprintf oc "(%a)@ha" symbol_offset (s, camlint_of_coqint n)
       end
   | Csymbol_sda(s, n) ->
-      assert false  (* treated specially in ireg_with_offset below *)
+      begin match target with
+      | Diab ->
+          fprintf oc "(%a)@sdarx" symbol_offset (s, camlint_of_coqint n)
+      | _ ->
+          assert false
+      end
+
 
 let num_crbit = function
   | CRbit_0 -> 0
@@ -164,20 +170,6 @@ let creg oc r =
   | MacOS|Diab -> fprintf oc "cr%d" r
   | Linux      -> fprintf oc "%d" r
 
-let ireg_with_offset oc (r, cst) =
-  match cst with
-  | Csymbol_sda(s, n) ->
-      begin match target with
-      | MacOS ->
-          assert false
-      | Linux ->
-          fprintf oc "(%a)@sdarel(%a)" symbol_offset (s, camlint_of_coqint n) ireg r
-      | Diab ->
-          fprintf oc "(%a)@sdarx(r0)" symbol_offset (s, camlint_of_coqint n)
-      end
-  | _ ->
-      fprintf oc "%a(%a)" constant cst ireg r
-
 let section oc name =
   fprintf oc "	%s\n" name
 
@@ -195,7 +187,7 @@ let (text, data, const_data, sdata, float_literal) =
       (".text",
        ".data",
        ".rodata",
-       ".section	.sdata,\"aw\",@progbits",
+       ".data",  (* unused *)
        ".section	.rodata.cst8,\"aM\",@progbits,8")
   | Diab ->
       (".text",
@@ -368,11 +360,11 @@ let print_instruction oc labels = function
       fprintf oc "%a:	.long	0x43300000, 0x00000000\n" label lbl;
       section oc text
   | Plbz(r1, c, r2) ->
-      fprintf oc "	lbz	%a, %a\n" ireg r1 ireg_with_offset (r2, c)
+      fprintf oc "	lbz	%a, %a(%a)\n" ireg r1 constant c ireg r2
   | Plbzx(r1, r2, r3) ->
       fprintf oc "	lbzx	%a, %a, %a\n" ireg r1 ireg r2 ireg r3
   | Plfd(r1, c, r2) ->
-      fprintf oc "	lfd	%a, %a\n" freg r1 ireg_with_offset (r2, c)
+      fprintf oc "	lfd	%a, %a(%a)\n" freg r1 constant c ireg r2
   | Plfdx(r1, r2, r3) ->
       fprintf oc "	lfdx	%a, %a, %a\n" freg r1 ireg r2 ireg r3
   | Plfi(r1, c) ->
@@ -386,19 +378,19 @@ let print_instruction oc labels = function
       fprintf oc "%a:	.long	0x%lx, 0x%lx\n" label lbl nhi nlo;
       section oc text
   | Plfs(r1, c, r2) ->
-      fprintf oc "	lfs	%a, %a\n" freg r1 ireg_with_offset (r2, c)
+      fprintf oc "	lfs	%a, %a(%a)\n" freg r1 constant c ireg r2
   | Plfsx(r1, r2, r3) ->
       fprintf oc "	lfsx	%a, %a, %a\n" freg r1 ireg r2 ireg r3
   | Plha(r1, c, r2) ->
-      fprintf oc "	lha	%a, %a\n" ireg r1 ireg_with_offset (r2, c)
+      fprintf oc "	lha	%a, %a(%a)\n" ireg r1 constant c ireg r2
   | Plhax(r1, r2, r3) ->
       fprintf oc "	lhax	%a, %a, %a\n" ireg r1 ireg r2 ireg r3
   | Plhz(r1, c, r2) ->
-      fprintf oc "	lhz	%a, %a\n" ireg r1 ireg_with_offset (r2, c)
+      fprintf oc "	lhz	%a, %a(%a)\n" ireg r1 constant c ireg r2
   | Plhzx(r1, r2, r3) ->
       fprintf oc "	lhzx	%a, %a, %a\n" ireg r1 ireg r2 ireg r3
   | Plwz(r1, c, r2) ->
-      fprintf oc "	lwz	%a, %a\n" ireg r1 ireg_with_offset (r2, c)
+      fprintf oc "	lwz	%a, %a(%a)\n" ireg r1 constant c ireg r2
   | Plwzx(r1, r2, r3) ->
       fprintf oc "	lwzx	%a, %a, %a\n" ireg r1 ireg r2 ireg r3
   | Pmfcrbit(r1, bit) ->
@@ -445,25 +437,25 @@ let print_instruction oc labels = function
   | Psrw(r1, r2, r3) ->
       fprintf oc "	srw	%a, %a, %a\n" ireg r1 ireg r2 ireg r3
   | Pstb(r1, c, r2) ->
-      fprintf oc "	stb	%a, %a\n" ireg r1 ireg_with_offset (r2, c)
+      fprintf oc "	stb	%a, %a(%a)\n" ireg r1 constant c ireg r2
   | Pstbx(r1, r2, r3) ->
       fprintf oc "	stbx	%a, %a, %a\n" ireg r1 ireg r2 ireg r3
   | Pstfd(r1, c, r2) ->
-      fprintf oc "	stfd	%a, %a\n" freg r1 ireg_with_offset (r2, c)
+      fprintf oc "	stfd	%a, %a(%a)\n" freg r1 constant c ireg r2
   | Pstfdx(r1, r2, r3) ->
       fprintf oc "	stfdx	%a, %a, %a\n" freg r1 ireg r2 ireg r3
   | Pstfs(r1, c, r2) ->
       fprintf oc "	frsp	%a, %a\n" freg FPR13 freg r1;
-      fprintf oc "	stfs	%a, %a\n" freg FPR13 ireg_with_offset (r2, c)
+      fprintf oc "	stfs	%a, %a(%a)\n" freg FPR13 constant c ireg r2
   | Pstfsx(r1, r2, r3) ->
       fprintf oc "	frsp	%a, %a\n" freg FPR13 freg r1;
       fprintf oc "	stfsx	%a, %a, %a\n" freg FPR13 ireg r2 ireg r3
   | Psth(r1, c, r2) ->
-      fprintf oc "	sth	%a, %a\n" ireg r1 ireg_with_offset (r2, c)
+      fprintf oc "	sth	%a, %a(%a)\n" ireg r1 constant c ireg r2
   | Psthx(r1, r2, r3) ->
       fprintf oc "	sthx	%a, %a, %a\n" ireg r1 ireg r2 ireg r3
   | Pstw(r1, c, r2) ->
-      fprintf oc "	stw	%a, %a\n" ireg r1 ireg_with_offset (r2, c)
+      fprintf oc "	stw	%a, %a(%a)\n" ireg r1 constant c ireg r2
   | Pstwx(r1, r2, r3) ->
       fprintf oc "	stwx	%a, %a, %a\n" ireg r1 ireg r2 ireg r3
   | Psubfc(r1, r2, r3) ->
