extraction/extraction.v
@@ -73,7 +73,6 @@ Extract Constant Linearize.enumerate_aux => "Linearizeaux.enumerate_aux".
 Extract Constant Asm.low_half => "fun _ -> assert false".
 Extract Constant Asm.high_half => "fun _ -> assert false".
 Extract Constant Asm.symbol_is_small_data => "Cil2Csyntax.atom_is_small_data".
-Extract Constant Asm.small_data_area_base => "fun _ -> assert false".
 Extract Constant Asm.small_data_area_offset => "fun _ _ _ -> assert false".
 
 (* Suppression of stupidly big equality functions *)
